moving new framework to Smt/Reconstruction

Reconstruction/BoolsExample.lean
@@ -1,21 +1,11 @@
-import Cdclt.Term
-import Cdclt.Boolean
+import Smt.Reconstruction.Term
 
 open proof
 open term
-open rules
-
-def beq  (b₁ b₂ : Bool) : Bool := b₁ == b₂
-def bneq (b₁ b₂ : Bool) : Bool := b₁ != b₂
 
 @[simp] def bimplies : Bool → Bool → Bool
 | true, false => false
 | _,    _     => true
-
-def bimplies' (x y : Bool) := !x || y
-
-#eval bimplies true false
-#eval bimplies' false true
 
 def Interpretation: Type := Nat → Bool
 
@@ -26,8 +16,8 @@ def Interpretation: Type := Nat → Bool
   | term.and     t₁ t₂ => and (interpTerm f t₁) (interpTerm f t₂)
   | term.or      t₁ t₂ => or (interpTerm f t₁) (interpTerm f t₂)
   | term.implies t₁ t₂ => bimplies (interpTerm f t₁) (interpTerm f t₂)
-  | term.xor     t₁ t₂ => bneq (interpTerm f t₁) (interpTerm f t₂)
-  | term.eq      t₁ t₂ => beq  (interpTerm f t₁) (interpTerm f t₂)
+  | term.xor     t₁ t₂ => (interpTerm f t₁) != (interpTerm f t₂)
+  | term.eq      t₁ t₂ => (interpTerm f t₁) == (interpTerm f t₂)
   | term.bot           => false
   | term.top           => true
   | _                  => false
@@ -37,7 +27,7 @@ def followsFrom (t₁ t₂ : term) : Prop :=
 
 -- Boolean rules
 
-theorem notImplies1' : ∀ {t₁ t₂ : term},
+theorem notImplies1 : ∀ {t₁ t₂ : term},
   followsFrom (not $ implies t₁ t₂) t₁
   | t₁, t₂, f, h =>
     match r₁: interpTerm f t₁, r₂: interpTerm f t₂ with
@@ -58,9 +48,9 @@ theorem interpNotTerm : ∀ {f : Interpretation} {t : term},
                   rewrite [r] at h
                   simp at h
 
-theorem notImplies2' : ∀ {t₁ t₂ : term},
+theorem notImplies2 : ∀ {t₁ t₂ : term},
   followsFrom (not $ implies t₁ t₂) (not t₂)
-  | t₁, t₂, f, h => have r₁ := notImplies1' h
+  | t₁, t₂, f, h => have r₁ := notImplies1 h
     match r₂: interpTerm f (not t₂) with
     | true  => rfl
     | false => by simp at h
@@ -68,7 +58,7 @@ theorem notImplies2' : ∀ {t₁ t₂ : term},
                   rewrite [r₁, r₂'] at h
                   simp at h
 
-theorem impliesElim' : ∀ {t₁ t₂: term},
+theorem impliesElim : ∀ {t₁ t₂: term},
   followsFrom (implies t₁ t₂) (or (not t₁) t₂)
   | t₁, t₂, f, h =>
     match r₁: interpTerm f t₁, r₂: interpTerm f t₂ with
@@ -82,7 +72,7 @@ theorem impliesElim' : ∀ {t₁ t₂: term},
                          rewrite [r₁, r₂]
                          exact (Or.inr rfl)
 
-theorem contradiction': ∀ {t: term},
+theorem contradiction: ∀ {t: term},
   followsFrom (and (not t) t) bot
   | t, f, h => by simp at h
                   cases r: interpTerm f t with
@@ -91,7 +81,7 @@ theorem contradiction': ∀ {t: term},
                   | true  => rewrite [r] at h
                              simp at h
 
-theorem R1' : ∀ {t₁ t₂ : term},
+theorem R1 : ∀ {t₁ t₂ : term},
   followsFrom (and (or (not t₁) t₂) t₁) t₂
   | t₁, t₂, f, h =>
     match r₁: interpTerm f t₁, r₂: interpTerm f t₂ with
@@ -109,79 +99,22 @@ theorem conjunction: ∀ {t₁ t₂: term} {f: Interpretation},
                             rewrite [h₁, h₂]
                             exact (And.intro rfl rfl)
 
--- EUF Rules
-
-theorem beqImpEq {a b : Bool} : a == b → a = b := λ h =>
-  match a, b with
-  | true,  true  => rfl
-  | false, true  => by simp at h
-  | true,  false => by simp at h
-  | false, false => rfl
-
-theorem eqImpBeq {a b : Bool} : a = b → a == b := λ h =>
-  match a, b with
-  | true,  true  => rfl
-  | false, true  => by simp at h
-  | true,  false => by simp at h
-  | false, false => rfl
-
-theorem refl': ∀ {t: term} {f: Interpretation},
-  interpTerm f (eq t t) = true
-  | t, f => by simp
-               cases interpTerm f t with
-               | true => simp
-               | false => simp
-
-theorem beqSymm: ∀ {a b: Bool}, a == b → b == a :=
-  λ h => eqImpBeq (Eq.symm (beqImpEq h))
-
-theorem symm': ∀ {t₁ t₂: term} {f: Interpretation},
-  interpTerm f (eq t₁ t₂) → interpTerm f (eq t₂ t₁)
-  | _, _, _, h =>
-    by simp at *
-       exact beqSymm h
-
-theorem nBeqSymm: ∀ {a b : Bool}, a != b → b != a
-  | true,  true, h  => h
-  | true,  false, _ => by simp
-  | false, true, _  => by simp
-  | false, false, h => h
-
-theorem negSymm' : ∀ {t₁ t₂ : term} {f : Interpretation},
-  interpTerm f (not $ eq t₁ t₂) → interpTerm f (not $ eq t₂ t₁)
-  | _, _, _, h =>
-    by simp at *
-       exact nBeqSymm h
-
-theorem beqTrans: ∀ {a b c: Bool}, a == b → b == c → a == c :=
-  λ h₁ h₂ => eqImpBeq (Eq.trans (beqImpEq h₁) (beqImpEq h₂))
-
-theorem trans': ∀ {t₁ t₂ t₃: term} {f: Interpretation},
-  interpTerm f (eq t₁ t₂) → interpTerm f (eq t₂ t₃) → interpTerm f (eq t₁ t₃)
-  | _, _, _, _, h₁, h₂ =>
-    by simp at *
-       exact beqTrans h₁ h₂
-
--- axiom cong : ∀ {f₁ t₁ : term} {f₂ t₂ : term},
---   thHolds (eq f₁ f₂) → thHolds (eq t₁ t₂) →
---         thHolds (eq (app f₁ t₁) (app f₂ t₂))
-
--- Examples
+-- Example (modus ponens)
 
 def p: term := const 1000 boolSort
 def q: term := const 1001 boolSort
 def mpDE': term := implies p (implies (implies p q) q)
 def notMpDE: term := not mpDE'
 
-theorem th0' : followsFrom notMpDE bot :=
+theorem th0 : followsFrom notMpDE bot :=
   λ lean_a0 =>
-    have lean_s0 := notImplies2' lean_a0
-    have lean_s1 := notImplies1' lean_s0
-    have lean_s2 := impliesElim' lean_s1
-    have lean_s4 := notImplies1' lean_a0
-    have lean_s6 := R1' (conjunction lean_s2 lean_s4)
-    have lean_s9 := notImplies2' lean_s0
-    contradiction' (conjunction lean_s9 lean_s6)
+    have lean_s0 := notImplies2 lean_a0
+    have lean_s1 := notImplies1 lean_s0
+    have lean_s2 := impliesElim lean_s1
+    have lean_s4 := notImplies1 lean_a0
+    have lean_s6 := R1 (conjunction lean_s2 lean_s4)
+    have lean_s9 := notImplies2 lean_s0
+    contradiction (conjunction lean_s9 lean_s6)
 
 theorem followsBot : ∀ {t : term},
   followsFrom t bot → ∀ {f : Interpretation}, interpTerm f t = false
@@ -192,14 +125,13 @@ theorem followsBot : ∀ {t : term},
     | false => rfl
 
 theorem notMpDEFalse: ∀ {f: Interpretation}, interpTerm f notMpDE = false :=
-  followsBot th0'
+  followsBot th0
 theorem mpDETrue: ∀ {f: Interpretation}, interpTerm f mpDE' = true :=
   interpNotTerm notMpDEFalse
 
-def modusPonens (x y: Bool) : Bool := bimplies (and (bimplies x y) x) y
-def curryModusPonens (x y: Bool) : Bool := bimplies x (bimplies (bimplies x y) y)
+def modusPonens (x y: Bool) : Bool := bimplies x (bimplies (bimplies x y) y)
 
-theorem mp: ∀ {x y: Bool}, curryModusPonens x y = true 
+theorem mp: ∀ {x y: Bool}, modusPonens x y = true 
   | x, y => @mpDETrue λ n => if n == 1000 then x else y
 
 @[simp] def is_equiv (l l₁ l₂: term) := l = xor l₁ l₂
