Smt.lean
@@ -13,3 +13,6 @@ import Smt.Solver
 import Smt.String
 import Smt.Tactic
 import Smt.Term
+
+import Smt.Reconstruction.Term
+import Smt.Reconstruction.ModusPonens
